begin design of kinit

compiler/kernel-template/ml/primitives/KrakenBaseImpl.ml
@@ -1,63 +1,17 @@
-let explode s =
-  let rec loop i cs =
-    if i < 0 then
-      cs
-    else
-      loop (i - 1) (s.[i] :: cs)
-  in
-  loop (String.length s - 1) []
-
-let implode cs =
-  let s = String.create (List.length cs) in
-  let rec loop i = function
-    | c :: cs' ->
-        s.[i] <- c;
-        loop (i + 1) cs'
-    | [] -> s
-  in
-  loop 0 cs
-
-(* NOTE MlCoq.Ascii has least significant bit first *)
-
-let char_of_ascii = function
-  | MlCoq.Ascii (b1, b2, b3, b4, b5, b6, b7, b8) ->
-      Char.chr (
-        (if b1 then   1 else 0) lor
-        (if b2 then   2 else 0) lor
-        (if b3 then   4 else 0) lor
-        (if b4 then   8 else 0) lor
-        (if b5 then  16 else 0) lor
-        (if b6 then  32 else 0) lor
-        (if b7 then  64 else 0) lor
-        (if b8 then 128 else 0))
-
-let ascii_of_char c =
-  let c = Char.code c in
-  MlCoq.Ascii
-    ( c land   1 <> 0
-    , c land   2 <> 0
-    , c land   4 <> 0
-    , c land   8 <> 0
-    , c land  16 <> 0
-    , c land  32 <> 0
-    , c land  64 <> 0
-    , c land 128 <> 0
-    )
-
-let string_of_str s =
-  implode (List.map char_of_ascii s)
-
-let str_of_string s =
-  List.map ascii_of_char (explode s)
-
 let int_of_num n =
-  Char.code (char_of_ascii n)
+  Char.code (MlCoq.char_of_ascii n)
 
 let kroot =
   try
     Sys.getenv "KROOT"
   with Not_found ->
-    failwith "KROOT environment variable is not set"
+    failwith "KROOT environment variable not set"
+
+let prog_path p =
+  List.fold_left
+    Filename.concat
+    ""
+    [kroot; "client"; p]
 
 (* Forked components need to know which file descriptor to use for
  * communicating with the kernel.
@@ -81,28 +35,37 @@ let string_of_fd fd =
  *)
 
 type chan = Unix.file_descr
-type fdesc = Unix.file_descr
 
 let chan_eq c1 c2 =
   c1 = c2
 
-(* TODO *)
-let exec s _ =
-  Unix.stdin
+type fdesc = Unix.file_descr
 
-(* prog path is relative to $KROOT/client *)
+let exec prog _ =
+  let prog = MlCoq.string_of_str prog in
+  let p, c = Unix.socketpair Unix.PF_UNIX Unix.SOCK_STREAM 0 in
+  match Unix.fork () with
+  | 0 -> (* child *) begin
+      Unix.close p;
+      let p = prog_path prog in
+      Unix.handle_unix_error (fun _ ->
+        Unix.execv p [|p; string_of_fd c|]) ()
+  end
+  | cpid -> (* parent *) begin
+      Unix.close c;
+      p
+  end
+
 let call prog arg _ =
-  let prog = string_of_str prog in
-  let arg = string_of_str arg in
+  let prog = MlCoq.string_of_str prog in
+  let arg = MlCoq.string_of_str arg in
   let r, w = Unix.pipe () in
   match Unix.fork () with
   | 0 -> (* child *) begin
       Unix.close r;
-      let prog =
-        List.fold_left Filename.concat "" [kroot; "client"; prog]
-      in
+      let p = prog_path prog in
       Unix.handle_unix_error (fun _ ->
-        Unix.execv prog [|prog; arg; string_of_fd w|]) ()
+        Unix.execv p [|p; arg; string_of_fd w|]) ()
   end
   | cpid -> (* parent *) begin
       Unix.close w;
@@ -110,24 +73,33 @@ let call prog arg _ =
   end
 
 let select chans _ =
-  let r, _, _ = Unix.select chans [] [] (-1.0) in
+  let r, _, _ =
+    Unix.handle_unix_error (fun _ ->
+      Unix.select chans [] [] (-1.0)) ()
+  in
   List.hd r
 
 let recv c n _ =
   let n = int_of_num n in
   let s = String.make n (Char.chr 0) in
-  let r = Unix.recv c s 0 n [] in
+  let r = 
+    Unix.handle_unix_error (fun _ ->
+      Unix.recv c s 0 n []) ()
+  in
   if r <> n then
-    failwith "recv"
+    failwith "recv - wrong # of bytes"
   else
-    str_of_string s
+    MlCoq.str_of_string s
 
 let send c s _ =
-  let s = string_of_str s in
+  let s = MlCoq.string_of_str s in
   let n = String.length s in
-  let w = Unix.send c s 0 n [] in
+  let w =
+    Unix.handle_unix_error (fun _ ->
+      Unix.send c s 0 n []) ()
+  in
   if w <> n then
-    failwith "send"
+    failwith "send - wrong # of bytes"
   else
     ()
 
@@ -136,23 +108,3 @@ let recv_fd c _ = recv_fd_native c
 
 external send_fd_native : chan -> fdesc -> unit = "send_fd_native"
 let send_fd c fd _ = send_fd_native c fd
-
-(*
- * TEMPORARY FOR TESTING
- *)
-
-let mkchan () =
-  let p, c = Unix.socketpair Unix.PF_UNIX Unix.SOCK_STREAM 0 in
-  match Unix.fork () with
-  | 0 -> (* child *) begin
-      Unix.close p;
-      let prog =
-        List.fold_left Filename.concat "" [kroot; "client"; "test.py"]
-      in
-      Unix.handle_unix_error (fun _ ->
-        Unix.execv prog [|prog; string_of_fd c|]) ()
-  end
-  | cpid -> (* parent *) begin
-      Unix.close c;
-      p
-  end
