compiler/kernel-template/coq/Extract.v
@@ -2,18 +2,16 @@ Require Import Ynot.Extract.
 Require Import KrakenBase.
 Require Import Kernel.
 
-Extract Constant KrakenBase.chan => "KrakenBaseImpl.chan".
+Extract Constant KrakenBase.chan    => "KrakenBaseImpl.chan".
 Extract Constant KrakenBase.chan_eq => "KrakenBaseImpl.chan_eq".
-Extract Constant KrakenBase.fdesc => "KrakenBaseImpl.fdesc".
-Extract Constant KrakenBase.exec => "KrakenBaseImpl.exec".
-Extract Constant KrakenBase.call => "KrakenBaseImpl.call".
-Extract Constant KrakenBase.select => "KrakenBaseImpl.select".
-Extract Constant KrakenBase.recv => "KrakenBaseImpl.recv".
-Extract Constant KrakenBase.send => "KrakenBaseImpl.send".
+Extract Constant KrakenBase.fdesc   => "KrakenBaseImpl.fdesc".
+Extract Constant KrakenBase.exec    => "KrakenBaseImpl.exec".
+Extract Constant KrakenBase.call    => "KrakenBaseImpl.call".
+Extract Constant KrakenBase.select  => "KrakenBaseImpl.select".
+Extract Constant KrakenBase.recv    => "KrakenBaseImpl.recv".
+Extract Constant KrakenBase.send    => "KrakenBaseImpl.send".
 Extract Constant KrakenBase.recv_fd => "KrakenBaseImpl.recv_fd".
 Extract Constant KrakenBase.send_fd => "KrakenBaseImpl.send_fd".
-
-Extract Constant Kernel.dummy => "KrakenBaseImpl.mkchan ()".
 
 Cd "../ml".
 Recursive Extraction Library Kernel.
